p2 example trying to preserve sharing using simp

Kraken/Examples.lean
@@ -37,6 +37,32 @@ example [layout : Layout] s : step1 (layout p1) (s, layout.start) (fun s => s.1.
 
   /- simp [p1,step1,eval1,fetch,Instr.is_ctrl,strt1,eval_operand,eval_imm,set_reg_or_mem,next,MachineState.setReg,Registers.set] -/
 
+def p2 := eval% parse! "start: mov $2, %rax
+dec %rax"
+
+-- Super-simple example to debug tactics
+example [layout : Layout] s : step1 (layout p2) (s, layout.start) (fun s => s.1.regs.rax = 1) := by
+  let ss := s
+  change (step1 _ (ss, _) _)
+  cases s with | mk regs flags mem =>
+  cases regs with | mk rax =>
+  delta p2
+  dsimp only [step1,Executable.straightline]
+  rw [Executable.directivesFromStart]
+  simp [List.mapIdx,List.mapIdx.go]
+  dsimp (zeta:=false) only [Directives.interp,Directive.interp,Instr.interp,Operation.interp,Operand.interp,ConstExpr.interp,RegOrMem.interp,Reg.interp,Reg64s.get,Reg.base,Reg.offset,MachineData.set,MachineData.setReg,Reg64s.set,Width.type,Width.bits]
+  dsimp (zeta:=false)(beta:=true)(eta:=false)(iota:=true)(proj:=true) only [Reg64s,get64,Reg64s.set64,BitVec.drop,BitVec.take,ss] -- reduces UInt64.toBitVec but leaves let binders behind and gets stuck confused on it
+  intros rax1
+  lift_lets; intros t -- unfortunately a separte tactic rather than a simp flag
+  -- simp [MachineData.regs,Reg64s.set64,Reg64s.get64,ss] at t -- made no progress for some reason
+  dsimp (zeta:=false)(beta:=false)(eta:=false)(iota:=false)(proj:=true) only [Reg64s.set64,Reg64s.get64,ss,t]
+  -- now just bashing because rax1 in context is already bad
+  simp [rax1]
+  dsimp (zeta:=false)(beta:=false)(eta:=false)(iota:=true)(proj:=true) only [Reg64s.set64,Reg64s.get64,ss,t]
+  dsimp
+  simp (ground:=True)
+  simp
+
 def swap : Program := eval% parse! "
   xor %rbx, %rax
   xor %rax, %rbx
